Sketch unification in sandbox/Simple.v

sandbox/Simple.v
@@ -1,76 +1,129 @@
+Require Import Coq.Program.Basics.
+Require Import Coq.Program.Equality.
+Require Import Coq.Setoids.Setoid.
+Require Import Coq.Classes.RelationClasses.
+Require Import Coq.Classes.Morphisms.
+Require Import Coq.Logic.Decidable.
+Require Import Coq.Bool.Bool.
 Require Import BohmTrees.
 
 (* for reference
-Inductive Term {Var : Set} : Set :=
+Inductive Term {Vs : Set} : Set :=
   | term_top : Term
   | term_bot : Term
   | term_join : Term -> Term -> Term
   | term_rand : Term -> Term -> Term
   | term_app : Term -> Term -> Term
-  | term_var : Var -> Term
-  | term_lambda : @Term (option Var) -> Term.
+  | term_var : Vs -> Term
+  | term_lambda : @Term (option Vs) -> Term.
 Arguments Term : default implicits.
 Hint Constructors Term.
 
-Inductive normal {Var : Set} : Term Var -> Prop :=
+Inductive normal {Vs : Set} : Term Vs -> Prop :=
   | normal_bot : normal BOT
   | normal_join x y : normal x -> normal y -> normal (x || y)
   | normal_rand x y : normal x -> normal y -> normal (x (+) y)
   | normal_app x y : inert x -> normal y -> normal (x * y)
-  | normal_lambda x : @normal (option Var) x -> normal (LAMBDA x)
+  | normal_lambda x : @normal (option Vs) x -> normal (LAMBDA x)
   | normal_var v : normal (VAR v)
-with inert {Var : Set} : Term Var -> Set :=
+with inert {Vs : Set} : Term Vs -> Set :=
   | inert_var v : inert (VAR v)
   | inert_app x y : inert x -> normal y -> inert (x * y).
 Hint Constructors normal inert.
 *)
 
-Inductive Normal {Var : Set} : Set :=
+Inductive Normal {Vs : Set} : Set :=
   | Normal_bot : Normal
   | Normal_join : Normal -> Normal -> Normal
   | Normal_rand : Normal -> Normal -> Normal
   | Normal_app : Inert -> Normal -> Normal
-  | Normal_lambda : @Normal (option Var) -> Normal
-  | Normal_var : Var -> Normal
-with Inert {Var : Set} : Set :=
-  | Inert_var : Var -> Inert
+  | Normal_lambda : @Normal (option Vs) -> Normal
+  | Normal_var : Vs -> Normal
+with Inert {Vs : Set} : Set :=
+  | Inert_var : Vs -> Inert
   | Inert_app : Inert -> Normal -> Inert.
 Hint Constructors Normal Inert.
 Arguments Normal : default implicits.
 Arguments Inert : default implicits.
 
-Inductive Tp {Var : Set} : Set :=
-  | Tp_any : Tp
+(*
+Fixpoint force_normal {Vs : Set} (t : Term Vs) : Normal Vs.  Admitted.
+Fixpoint forget_normal {Vs : Set} (n : Normal Vs) : Term Vs.  Admitted.
+Lemma force_forget {Vs : Set} (n : Normal Vs) :
+  force_normal (forget_normal n) = n.
+*)
+
+Inductive Tp {Vs : Set} : Set :=
+  | Tp_var : Vs -> Tp
   | Tp_exp : Tp -> Tp -> Tp
-  | Tp_var : Var -> Tp.
+  | Tp_hole : Tp
+  | Tp_error : Tp.
 Hint Constructors Tp.
 Arguments Tp : default implicits.
 
-Inductive TNormal {TVar Var : Set} : Set :=
-  | TNormal_bot : Tp TVar -> TNormal
-  | TNormal_join : Tp TVar -> TNormal -> TNormal -> TNormal
-  | TNormal_rand : Tp TVar -> TNormal -> TNormal -> TNormal
-  | TNormal_app : Tp TVar -> TInert -> TNormal -> TNormal
-  | TNormal_lambda : Tp TVar -> @TNormal TVar (option Var) -> TNormal
-  | TNormal_var : Tp TVar -> Var -> TNormal
-with TInert {TVar Var : Set} : Set :=
-  | TInert_var : Tp TVar -> Var -> TInert
-  | TInert_app : Tp TVar -> TInert -> TNormal -> TInert.
+Definition delta (Var : Set) := forall x y : Var, {x = y} + {~ x = y}.
+
+Definition sumbool_if {p q : Prop} {t : Type} : {p} + {q} -> t -> t -> t :=
+  fun b x y =>
+  match b with
+  | left _ => x
+  | right _ => y
+  end.
+
+(* TODO this does not specialize *)
+Fixpoint unify {Vs : Set} (d : delta Vs) (a b : Tp Vs) : Tp Vs :=
+  match a, b with
+  | Tp_hole, c => c
+  | c, Tp_hole => c
+  | Tp_var v, Tp_var v' => sumbool_if (d v v') a Tp_error
+  | Tp_exp a1 a2, Tp_exp b1 b2 =>
+    let c1 := unify d a1 b1 in
+    let c2 := unify d a2 b2 in
+    match c1, c2 with
+    | Tp_error, _ => Tp_error
+    | _, Tp_error => Tp_error
+    |_, _ => Tp_exp c1 c2
+    end
+  | _, _ => Tp_error
+  end.
+
+Inductive TNormal {Ts Vs : Set} : Set :=
+  | TNormal_bot : Tp Ts -> TNormal
+  | TNormal_join : Tp Ts -> TNormal -> TNormal -> TNormal
+  | TNormal_rand : Tp Ts -> TNormal -> TNormal -> TNormal
+  | TNormal_app : Tp Ts -> TInert -> TNormal -> TNormal
+  | TNormal_lambda : Tp Ts -> @TNormal Ts (option Vs) -> TNormal
+  | TNormal_var : Tp Ts -> Vs -> TNormal
+with TInert {Ts Vs : Set} : Set :=
+  | TInert_var : Tp Ts -> Vs -> TInert
+  | TInert_app : Tp Ts -> TInert -> TNormal -> TInert.
 Hint Constructors TNormal TInert.
 Arguments TNormal : default implicits.
 Arguments TInert : default implicits.
 
-Fixpoint annotate_any {TVar Var : Set} (n : Normal Var) : TNormal TVar Var :=
+Fixpoint annotate_any {Ts Vs : Set} (n : Normal Vs) : TNormal Ts Vs :=
   match n with
-  | Normal_bot => TNormal_bot Tp_any
-  | Normal_join x y => TNormal_join Tp_any (annotate_any x) (annotate_any y)
-  | Normal_rand x y => TNormal_rand Tp_any (annotate_any x) (annotate_any y)
-  | Normal_app x y => TNormal_app Tp_any (annotate_any' x) (annotate_any y)
-  | Normal_lambda x => TNormal_lambda Tp_any (annotate_any x)
-  | Normal_var v => TNormal_var Tp_any v
+  | Normal_bot => TNormal_bot Tp_hole
+  | Normal_join x y => TNormal_join Tp_hole (annotate_any x) (annotate_any y)
+  | Normal_rand x y => TNormal_rand Tp_hole (annotate_any x) (annotate_any y)
+  | Normal_app x y => TNormal_app Tp_hole (annotate_any' x) (annotate_any y)
+  | Normal_lambda x => TNormal_lambda Tp_hole (annotate_any x)
+  | Normal_var v => TNormal_var Tp_hole v
   end
-with annotate_any' {TVar Var : Set} (i : Inert Var) : TInert TVar Var :=
+with annotate_any' {Ts Vs : Set} (i : Inert Vs) : TInert Ts Vs :=
   match i with
-  | Inert_var v => TInert_var Tp_any v
-  | Inert_app x y => TInert_app Tp_any (annotate_any' x) (annotate_any y)
+  | Inert_var v => TInert_var Tp_hole v
+  | Inert_app x y => TInert_app Tp_hole (annotate_any' x) (annotate_any y)
   end.
+
+(* TODO
+Inductive inhabits {Ts Vs : Set} : Normal Vs -> Tp Ts -> Prop :=
+  | inhabits_bot t : inhabits Normal_bot t
+.
+
+Inductive infers {Ts Vs : Set} : relation (TNormal Ts Vs) :=
+  | infers_bot t : infers (TNormal_bot Tp_hole) (TNormal_bot t)
+  | infers_join t tx x ty y :
+      infers tx x
+.
+*)
